Balanced Growth Path and productivity process
========================================================

Along a deterministic Balanced Growth Path, consumption, output, capital and investment
growth at the same constant rate equal to $(1+\mu_a)$ . This justifies
defining stationary modifications of those variable as follows:

$$C_t := \frac{\tilde{C}_t}{A_{t-1}  }, \quad  K_t := \frac{\tilde{K}_t}{A_{t-1} }, \quad  I_t := \frac{\tilde{I}_t}{A_{t-1} }, \quad L_t := \tilde{L}_t$$

At times we will refer to these scaled variables as the stationary variables.

BGP rates 
---------

In a deterministic BGP , neutral productivity grows at a constant gross
rate of $(1+\mu_a)$. The fraction of hours devoted to work is
obviously bounded, so in a BGP it must be constant.

Call $r_y$ the net growth rate and
call $R_y := (1+r_y)$ to the gross growth rate of consumption and
output. *Suppose, now, that in a BGP the fraction of total output
devoted to consumption is constant*. The resource constraint (when binding) implies that investment, too,
will grow at rate $R_y$ in a BGP :
$$C_t + I_t = Y_t \quad \Rightarrow \quad  I_{t+1} = Y_{t+1} - C_{t+1} = R_y Y_{t} - R_y C_{t} = R_y (Y_{t} -  C_{t}) = R_y I_{t} = R_i I_{t} \Rightarrow R_i = R_y$$

Call $R_k$ the gross growth rate of capital in a BGP. Since investment
will grow at rate $R_y$,
the law of motion of capital implies that
$R_k =  R_y$
$$K_{t+1} =  R_y  ~ K_t$$

$$K_{t+1} = (1-\delta) K_{t} +    I_t$$
$$\Rightarrow  K_{t+2} = (1-\delta) K_{t+1} +    I_{t+1}$$
$$K_{t+1} R_k = (1-\delta)K_{t} R_k  +   I_{t} R_I $$
$$K_{t+1}  = (1-\delta)K_{t} R_k  +    I_{t} R_I  \frac{1}{R_k}$$
$$\Rightarrow   \frac{R_I }{R_k} = 1$$
$$\Rightarrow R_k = R_I  $$
$$\Rightarrow R_k = R_y  $$

Now that the growth rate of capital along the BGP ($R_k$) is written in
terms of that of product ($R_y$) and since $R_L = 1$, we could solve
$R_y$ in terms of modelâs parameters: Then, along the deterministic BGP:
$$\tY_t = A_{t}^{1-\alpha} \tK_t^{\alpha} L_t^{1-\alpha}$$
$$\tY_{t+1} = A_{t+1}^{1-\alpha} \tK_{t+1}^{\alpha} L_{t+1}^{1-\alpha}$$
$$\tY_{t} R_y = (1+\mu_a)^{1-\alpha} A_{t}^{1-\alpha} R_{k}^{\alpha} \tK_{t}^{\alpha} L_{t}^{1-\alpha}$$
$$\tY_{t} R_y = (1+\mu_a)^{1-\alpha} R_{k}^{\alpha} A_{t}^{1-\alpha}  \tK_{t}^{\alpha} L_{t}^{1-\alpha}$$
$$\tY_{t} R_y = (1+\mu_a)^{1-\alpha} R_{k}^{\alpha} \tY_t \$$
$$R_y = (1+\mu_a)^{1-\alpha} R_{k}^{\alpha}  \$$
$$R_y = (1+\mu_a)^{1-\alpha} [ R_{y}]^{\alpha}$$
$$R_y = [(1+\mu_a) ]^{1-\alpha} R_{y}^{\alpha}$$
$$R_y^{1-\alpha}  = [(1+\mu_a) ]^{1-\alpha}$$
$$R_y  = (1+\mu_a) $$

$$\Rightarrow R_k  =  (1+\mu_a)  = (1+\mu_a)$$

Then an obvious variable that growth a rate $R_y$ is $A_s$
and one that growth at rate $R_k$ is $A_s$ for any $s$.
